AllNotations.v
@@ -1,5 +1,7 @@
 Require Export Kami.AllDefn.
 Require Export Kami.Notations.
 Require Export Kami.LibStruct.
-Export Word.Notations.
+Require Export Kami.Lib.HexNotationWord.
+Require Kami.Lib.Word.
+Export Kami.Lib.Word.Notations.
 Export ListNotations.
