Tutorial/SyntaxEx.v
@@ -1,4 +1,5 @@
 Require Import Kami.AllNotations.
+Require Import ZArith.
 
 (* In order to write a Kami module, one first opens a section using the same name as the module,
   and writes the following five lines of boiler plate code. *)
